first work for preludes with fixed input

theories/L/Complexity/Cook/GenNP.v
@@ -1,12 +1,12 @@
 From Undecidability.TM Require Import TM.
 From Undecidability.L.TM Require Import TMflat TMflatEnc TMflatFun TMEncoding TapeDecode TMunflatten.
+From Undecidability.L.Complexity.Cook Require Import FlatFinTypes.
 
 (** *Definition of a generic NP-hard problem *)
 (*(at least it is NP-hard if one accepts Turing machines)*)
 
-(*we constrain the form the initial configuration of the Turing machine has:
- the head is required to stand left of the input*)
-Definition isValidInput (sig : finType) k (s : list sig) := |s| <= k. 
+Definition isValidCert (sig : finType) k' (c : list sig) := |c| <= k'.
+Definition isValidInput (sig : finType) s k' (inp : list sig) := exists c, isValidCert k' c /\ inp = s ++ c. 
 
 Definition initialTapeForString (sig : finType) (s : list sig) :=
   match s with
@@ -15,12 +15,11 @@ Definition initialTapeForString (sig : finType) (s : list sig) :=
   end. 
 
 (*single-tape machine whose head will always start at the leftmost position (i.e. initial tapes are niltape or leftof) *)
-Definition GenNP (i : { sig : finType & (mTM sig 1 * nat * nat)%type } ) : Prop := 
-  match i with existT _ sig (tm, k, t) => exists inp, |inp| <= k
-                                                      /\ exists f, loopM (initc tm ([|initialTapeForString inp|])) t = Some f
+Definition GenNP (i : { sig : finType & (mTM sig 1 * list sig * nat * nat)%type } ) : Prop := 
+  match i with existT _ sig (tm, s, k', t) => exists cert, |cert| <= k'
+                                                      /\ exists f, loopM (initc tm ([|initialTapeForString (s ++ cert)|])) t = Some f
   end.
 
-Definition FlatGenNP : TM*nat*nat -> Prop:=
-  fun '(M,maxSize, steps (*in unary*)) =>
-    exists sig (M':mTM sig 1), isFlatteningTMOf M M' /\ GenNP (existT _ _ (M', maxSize, steps)). 
-
+Definition FlatGenNP : TM*list nat *nat*nat -> Prop:=
+  fun '(M,s,maxSize, steps (*in unary*)) =>
+    exists sig (M':mTM sig 1) sfin, isFlatteningTMOf M M' /\ isFlatListOf s sfin /\ GenNP (existT _ _ (M', sfin, maxSize, steps)). 
